More implementation.

pulse/lib/pulse/core/PulseCore.IndirectionTheorySep.fst
@@ -3,21 +3,23 @@ module I = PulseCore.IndirectionTheorySepImpl
 open FStar.Ghost
 module PropExt = FStar.PropositionalExtensionality
 
+[@@erasable]
 noeq type istore = {
-  ist: (is:I.istore { I.istore_slprops_ok is });
+  ist: I.okay_istore;
   saved_credits: erased nat;
   freshness_counter: nat;
 }
 
+[@@erasable]
 noeq type core_istore = {
-  ist: (is:I.istore { I.istore_slprops_ok is });
+  ist: I.okay_istore;
   saved_credits: erased nat;
 }
 
-// let to_core (w: I.world) : core_istore =
-//   { ist = fst w; saved_credits = (snd w).saved_credits; pulse_mem = (snd w).pulse_heap }
+let to_core (w: I.world) : core_mem =
+  { istore = { ist = fst w; saved_credits = (snd w).saved_credits }; pulse_mem = (snd w).pulse_heap }
 
-let of_core (m: core_mem) : I.world =
+let of_core (m: core_mem) : GTot I.world =
   (m.istore.ist, ({ saved_credits = m.istore.saved_credits; pulse_heap = m.pulse_mem } <: I.rest))
 
 let istore_core i = { ist = i.ist; saved_credits = i.saved_credits }
@@ -27,13 +29,19 @@ let age1 k =
 
 let slprop = I.slprop
 
+let ilevel k = I.level_istore k.ist
 let level k = I.level_istore k.istore.ist
 
-let credits k = k.saved_credits
+let level_depends_on_core_istore_only m = ()
 
-let is_ghost_action_istore = admit ()
+let icredits k = k.saved_credits
 
-let update_ghost = admit ()
+let is_ghost_action_istore i1 i2 =
+  i1.saved_credits >= i2.saved_credits /\
+  i1.freshness_counter <= i2.freshness_counter
+
+let update_ghost m1 m2 =
+  { istore = (reveal m2).istore; pulse_mem = PM.pulse_heap_sig.update_ghost m1.pulse_mem (reveal m2).pulse_mem; }
 
 let emp = I.emp
 let pure = I.pure
@@ -49,6 +57,8 @@ let istore_join i0 i1 =
   { ist = I.join_istore i0.ist i1.ist; saved_credits = i0.saved_credits + i1.saved_credits }
 
 let istore_join_refl i = I.join_istore_refl i.ist
+
+let disjoint_join_levels i0 i1 = ()
 
 let interp p =
   introduce forall (m0 m1:core_mem). p (of_core m0) /\ disjoint m0 m1 ==> p (of_core (join m0 m1)) with
@@ -74,9 +84,63 @@ let lift_exists_eq a f =
 
 let iref = I.iref
 let deq_iref = fun x y -> reveal x = reveal y
-let lower_inames = admit()
+let lower_inames i = GhostSet.empty
 
 let istore_inames_ok e m = admit ()
 
 let inames_ok_empty m = admit ()
 let inames_ok_union m = admit ()
+
+let istore_invariant ex i = admit ()
+
+let inv i p = I.inv i p
+
+let later p = I.later p
+let later_credit n = I.later_credit n
+let equiv = I.equiv
+
+let intro_later p m = ()
+
+let istore_dom m = I.istore_dom m.istore.ist
+
+let pulse_ghost_action_refl m : Lemma (PM.is_ghost_action m m) [SMTPat (PM.is_ghost_action m m)] =
+  PM.pulse_heap_sig.is_ghost_action_preorder ()
+
+let age_mem m =
+  let m': mem = { m with istore = { m.istore with ist = I.age1_istore m.istore.ist } } in
+  GhostSet.lemma_equal_intro (istore_dom m) (istore_dom m'); assert istore_dom m == istore_dom m';
+  m'
+
+let age_level m = ()
+
+let age_disjoint m0 m1 = ()
+
+let age_hereditary p m =
+  assert of_core (age1 m) == I.age1_ (of_core m)
+
+let age_later p m = ()
+
+let spend m =
+  { m with istore = { m.istore with
+    saved_credits = if m.istore.saved_credits > 0 then m.istore.saved_credits - 1 else 0 } }
+
+let spend_mem m =
+  { m with istore = { m.istore with
+    saved_credits = if m.istore.saved_credits > 0 then m.istore.saved_credits - 1 else 0 } }
+
+let interp_later_credit n m = ()
+
+let spend_lemma m = ()
+
+let spend_disjoint m0 m1 = ()
+
+let buy n m = { m with istore = { m.istore with saved_credits = m.istore.saved_credits + n } }
+let buy_mem n m = { m with istore = { m.istore with saved_credits = m.istore.saved_credits + n } }
+let buy_lemma n m = ()
+let buy_disjoint n m0 m1 = ()
+
+let mem_invariant_equiv e m i p = admit ()
+
+let istore_dom = admit ()
+
+let inames_ok_istore_dom e m = admit ()
